Embed P256 in Spec.Agile.DH

specs/Spec.Agile.DH.fst
@@ -11,25 +11,32 @@ open Lib.ByteSequence
 type algorithm =
   | DH_Curve25519
   | DH_Curve448
+  | DH_P256
 
 inline_for_extraction
 let size_key (a:algorithm) : Tot size_nat =
   match a with
   | DH_Curve25519 -> 32
   | DH_Curve448 -> 56
+  | DH_P256 -> 32
 
+inline_for_extraction
+let size_public (a:algorithm) : Tot size_nat =
+  match a with
+  | DH_Curve25519 -> 32
+  | DH_Curve448 -> 56
+  | DH_P256 -> 64
 
 /// Types
 
-type key (a:algorithm) = lbytes (size_key a)
 type scalar (a:algorithm) = lbytes (size_key a)
-type serialized_point (a:algorithm) = lbytes (size_key a)
+type serialized_point (a:algorithm) = lbytes (size_public a)
 
 
 /// Functions
 
 val scalarmult:
-    a:algorithm{a == DH_Curve25519 \/ a == DH_Curve448}
+    a:algorithm
   -> k:scalar a
   -> u:serialized_point a ->
   Tot (serialized_point a)
@@ -38,21 +45,26 @@ let scalarmult a k u =
   match a with
   | DH_Curve25519 -> Spec.Curve25519.scalarmult k u
   | DH_Curve448 -> Spec.Curve448.scalarmult k u
+  | DH_P256 -> Spec.P256.scalarmult k u
 
+#set-options "--z3rlimit 50"
 
-val dh: a:algorithm -> k0:key a -> k1:key a -> Tot (option (key a))
-let dh a k0 k1 =
-  let secret =
+val dh: a:algorithm -> s:scalar a -> p:serialized_point a -> Tot (option (serialized_point a))
+let dh a s p =
+  let output = scalarmult a s p in
+  let result : bool =
     match a with
-    | DH_Curve25519 -> scalarmult a k0 k1
-    | DH_Curve448 -> scalarmult a k0 k1
+    | DH_Curve25519 | DH_Curve448 -> not (lbytes_eq (create (size_public a) (u8 0)) output)
+    | DH_P256 ->
+      let r = Spec.P256.serialized_to_point output in
+      (Spec.P256.isPointOnCurve r && (not (Spec.P256.isPointAtInfinity r)))
   in
-  let result : bool = not (lbytes_eq (create (size_key a) (u8 0)) secret) in
-  if result then Some secret else None
+  if result then Some output else None
 
 
-val secret_to_public: a:algorithm -> key a -> Tot (key a)
+val secret_to_public: a:algorithm -> scalar a -> Tot (serialized_point a)
 let secret_to_public a kpriv =
   match a with
   | DH_Curve25519 -> Spec.Curve25519.secret_to_public kpriv
   | DH_Curve448 -> Spec.Curve448.secret_to_public kpriv
+  | DH_P256 -> Spec.P256.secret_to_public kpriv
